Add support for interaction with files
We now support the `--hints-file` and `--output-asm` arguments (both
unused) and the `--output` / `-o` argument.  The first two are initial
support for interacting with assembly hint files, though we don't
currently do anything with the arguments other than opening and reading
the files, and parsing the assembly.

src/Assembly/Parse.v
@@ -317,19 +317,117 @@ Global Instance show_lines_Lines : ShowLines Lines
 
 Definition parse_correct_on (v : list string)
   := forall res, parse v = Success res -> parse v = parse (show_lines false res).
-Definition parse_correct_on_bool (v : list string) : bool
+
+Inductive ParseError :=
+| Parse_error (msgs : list string)
+.
+
+Inductive ParseValidatedError :=
+| Initial_parse_error (err : ParseError)
+| Reparse_error (new_asm : list string) (err : ParseError)
+| Lengths_not_equal (old_asm : Lines) (new_asm : Lines)
+| Lines_not_equal (mismatched_lines : list (Line * Line))
+.
+Global Coercion Initial_parse_error : ParseError >-> ParseValidatedError.
+
+Global Instance show_lines_ParseError : ShowLines ParseError
+  := fun parens err => match err with
+                       | Parse_error err => err
+                       end.
+Global Instance show_ParseError : Show ParseError
+  := fun parens err => String.concat String.NewLine (show_lines parens err).
+Global Instance show_lines_ParseValidatedError : ShowLines ParseValidatedError
+  := fun parens err => match err with
+                       | Initial_parse_error err
+                         => match show_lines parens err with
+                            | [] => ["Unknown error while parsing assembly"]
+                            | [err] => ["Error while parsing assembly: " ++ err]%string
+                            | lines => "Error while parsing assembly:" :: lines
+                            end
+                       | Reparse_error new_asm err
+                         => match show_lines parens err with
+                            | [] => ["Unknown error while reparsing assembly:"] ++ new_asm
+                            | [err] => (["Error while reparsing assembly: " ++ err
+                                         ; "New assembly being parsed:"]%string)
+                                         ++ new_asm
+                            | lines => ["Error while parsing assembly:"]
+                                         ++ lines
+                                         ++ [""]
+                                         ++ ["New assembly being parsed:"]
+                                         ++ new_asm
+                            end
+                       | Lengths_not_equal old_asm new_asm
+                         => ["Reparsing the assembly:"]
+                              ++ show_lines parens old_asm
+                              ++ [""]
+                              ++ ["Yielded non-equal assembly:"]
+                              ++ show_lines parens new_asm
+                              ++ [""]
+                              ++ (["The number of lines was not equal (" ++ show false (List.length old_asm) ++ " ≠ " ++ show false (List.length new_asm) ++ ")"]%string)
+                       | Lines_not_equal mismatched_lines
+                         => ["When reparsing assembly for validation, the following lines were not equal:"]
+                              ++ (List.flat_map (fun '(old, new) => ["- " ++ show false old; "+ " ++ show false new; ""]%string)
+                                                mismatched_lines)
+                       end%list.
+Global Instance show_ParseValidatedError : Show ParseValidatedError
+  := fun parens err => String.concat String.NewLine (show_lines parens err).
+
+Definition parse_validated (v : list string) : ErrorT ParseValidatedError Lines
   := match parse v with
-     | Success res => match parse (show_lines false res) with
-                      | Success res' => Lines_beq res res'
-                      | Error _ => false
-                      end
-     | Error _ => true
+     | Success v
+       => let new_asm := show_lines false v in
+          match parse new_asm with
+          | Success v'
+            => if (List.length v =? List.length v')%nat
+               then match List.filter (fun '(x, y) => negb (Line_beq x y)) (List.combine v v') with
+                    | nil => Success v
+                    | mismatched_lines => Error (Lines_not_equal mismatched_lines)
+                    end
+               else Error (Lengths_not_equal v v')
+          | Error e
+            => Error (Reparse_error new_asm (Parse_error e))
+          end
+     | Error e => Error (Initial_parse_error (Parse_error e))
      end.
+
+Definition parse_correct_on_bool (v : list string) : bool
+  := match parse v, parse_validated v with
+     | Success _, Success _ => true
+     | Error _, _ => true
+     | Success _, Error _ => false
+     end.
+
+Definition parse_validated_correct_on v
+  := forall res, parse_validated v = Success res <-> parse v = Success res.
+
+Lemma parse_validated_correct_on_iff v : parse_validated_correct_on v <-> parse_correct_on v.
+Proof.
+  cbv [parse_validated_correct_on parse_correct_on parse_validated].
+  destruct (parse_Lines v) eqn:Hp; [ | split; [ congruence | split; congruence ] ].
+  destruct (parse_Lines (show_lines false _)) eqn:Hp2; (split; [ intros H res Hres; inversion Hres; subst | intro H; specialize (H _ eq_refl); rewrite <- H in Hp2; inversion Hp2; subst ]); rewrite ?Nat.eqb_refl, ?combine_same; try congruence.
+  all: repeat first [ progress destruct_head' iff
+                    | congruence
+                    | progress subst
+                    | progress rewrite ?Nat.eqb_eq in *
+                    | match goal with
+                      | [ H : forall x, _ <-> Success ?y = Success x |- _ ] => specialize (H y)
+                      | [ H : ?x = ?x |- _ ] => clear H
+                      | [ H : Success ?x = Success ?y |- _ ] => inversion H; clear H
+                      | [ H : ?x = ?x -> _ |- _ ] => specialize (H eq_refl)
+                      end
+                    | break_innermost_match_hyps_step
+                    | progress break_match_hyps
+                    | progress break_match
+                    | progress intros
+                    | apply conj ].
+Abort.
+
 Lemma parse_correct_on_bool_iff v : parse_correct_on_bool v = true <-> parse_correct_on v.
 Proof.
-  cbv [parse_correct_on_bool parse_correct_on].
-  destruct (parse_Lines v) eqn:Hp; [ | split; [ congruence | reflexivity ] ].
-  destruct (parse_Lines (show_lines false _)) eqn:Hp2; (split; [ intros H res Hres; inversion Hres; subst | intro H; specialize (H _ eq_refl); rewrite <- H in Hp2; inversion Hp2; subst ]); try congruence.
+  assert (parse_validated_correct_on_iff : forall v, parse_validated_correct_on v <-> parse_correct_on v) by admit.
+  rewrite <- parse_validated_correct_on_iff.
+  cbv [parse_correct_on_bool parse_validated_correct_on].
+  destruct (parse_Lines v) eqn:Heq1, (parse_validated v) eqn:Heq2; split; try split; try congruence.
 Abort.
 
 (* This version allows for easier debugging because it highlights the differences *)
